src/SymILProofs.v
@@ -1,0 +1,489 @@
+(** This file implements symbolic evaluation for the
+ ** language defined in IL.v
+ **)
+Require Import IL SepIL.
+Require Import Word Memory.
+Require Import DepList EqdepClass.
+Require Import PropX.
+Require Import SepExpr SymEval.
+Require Import Expr.
+Require Import Prover.
+Require Import Env TypedPackage.
+Import List.
+
+Require Structured SymEval.
+Require Import ILEnv SymIL.
+
+Set Implicit Arguments.
+Set Strict Implicit.
+
+(** The Symbolic Evaluation Interfaces *)
+Module MEVAL := SymIL.MEVAL.
+
+Module SymIL_Correct.
+  Section typed.
+    Variable ts : list type.
+    Let types := repr bedrock_types_r ts.
+
+    Local Notation "'pcT'" := (tvType 0).
+    Local Notation "'tvWord'" := (tvType 0).
+    Local Notation "'stT'" := (tvType 1).
+    Local Notation "'tvState'" := (tvType 2).
+    Local Notation "'tvTest'" := (tvType 3).
+    Local Notation "'tvReg'" := (tvType 4).
+
+    Variable fs : functions types.
+    Let funcs := repr (bedrock_funcs_r ts) fs.
+    Variable preds : SEP.predicates types pcT stT.
+
+    Variable Prover : ProverT types.
+    Variable PC : ProverT_correct Prover funcs.
+
+    Variable meval : MEVAL.MemEvaluator types pcT stT.
+    Variable meval_correct : MEVAL.MemEvaluator_correct meval funcs preds tvWord tvWord
+      (@IL_mem_satisfies ts) (@IL_ReadWord ts) (@IL_WriteWord ts).
+
+    Variable facts : Facts Prover.
+    Variable meta_env : env types.
+    Variable vars_env : env types.
+
+    Ltac t_correct := 
+      simpl; intros;
+        unfold IL_stn_st, IL_mem_satisfies, IL_ReadWord, IL_WriteWord in *;
+          repeat (simpl in *; 
+            match goal with
+              | [ H : Some _ = Some _ |- _ ] => inversion H; clear H; subst
+              | [ H : prod _ _ |- _ ] => destruct H
+              | [ H : match ?X with 
+                        | Some _ => _
+                        | None => _ 
+                      end |- _ ] =>
+              revert H; case_eq X; intros; try contradiction
+              | [ H : match ?X with 
+                        | Some _ => _
+                        | None => _ 
+                      end = _ |- _ ] =>
+              revert H; case_eq X; intros; try congruence
+              | [ H : _ = _ |- _ ] => rewrite H
+              | [ H : reg |- _ ] => destruct H
+            end; intuition); subst.
+
+    Lemma sym_evalLoc_correct : forall loc ss res res' stn_st locD cs,
+      stateD funcs preds meta_env vars_env cs stn_st ss ->
+      sym_locD funcs meta_env vars_env loc = Some locD ->
+      evalLoc (snd stn_st) locD = res' ->
+      sym_evalLoc loc ss = res -> 
+      exprD funcs meta_env vars_env res tvWord = Some res'.
+    Proof.
+      destruct loc; unfold stateD; destruct ss; destruct SymRegs; destruct p; subst funcs; t_correct.
+    Qed.
+    
+    Hypothesis Valid_facts : Valid PC meta_env vars_env facts.
+    
+    Lemma sym_evalRval_correct : forall rv ss res stn_st rvD cs,
+      stateD funcs preds meta_env vars_env cs stn_st ss ->
+      sym_rvalueD funcs meta_env vars_env rv = Some rvD ->
+      sym_evalRval Prover meval facts rv ss = Some res ->
+      exists val,
+        evalRvalue (fst stn_st) (snd stn_st) rvD = Some val /\
+        exprD funcs meta_env vars_env res tvWord = Some val.
+    Proof.
+      destruct rv; unfold stateD; t_correct; try congruence;
+        try solve [ destruct ss; destruct SymRegs; destruct p; intuition; t_correct; eauto ].
+
+      destruct s; t_correct; destruct ss; destruct SymRegs; destruct p; intuition; t_correct; eauto.
+      t_correct;
+      match goal with
+        | [ H : MEVAL.smemeval_read_word _ _ _ _ _ = _ |- _ ] => 
+          eapply (MEVAL.ReadCorrect meval_correct) in H; eauto; t_correct
+      end; eauto.
+      eapply sym_evalLoc_correct with (cs := cs); eauto. instantiate (1 := (s0, s1)). t_correct.
+      reflexivity.
+      congruence.
+    Qed.
+          
+    Lemma sym_evalLval_correct : forall lv stn_st lvD cs val ss ss' valD,
+      stateD funcs preds meta_env vars_env cs stn_st ss ->
+      sym_lvalueD funcs meta_env vars_env lv = Some lvD ->
+      sym_evalLval Prover meval facts lv val ss = Some ss' ->
+      exprD funcs meta_env vars_env val tvWord = Some valD ->
+      exists st', 
+        evalLvalue (fst stn_st) (snd stn_st) lvD valD = Some st' /\
+        stateD funcs preds meta_env vars_env cs (fst stn_st, st') ss'.
+    Proof.
+      destruct lv.
+        Focus.
+        destruct ss; destruct SymRegs; destruct p. unfold funcs in *.
+          t_correct; eexists; repeat (split; try reflexivity; eauto);
+            try solve [ repeat rewrite sepFormula_eq in *; unfold sepFormula_def in *; simpl in *; auto ].
+
+        Focus.
+        unfold funcs in *.
+        t_correct.
+        eapply sym_evalLoc_correct with (stn_st := (s0, s1)) in H0; simpl in *; eauto.
+        destruct ss; intuition. destruct SymRegs. destruct p. simpl in *. subst. intuition.
+        repeat match type of H1 with
+                 | match ?X with | Some _ => _ | None => _ end => destruct X; try contradiction
+               end.            
+        match goal with
+          | [ H : MEVAL.smemeval_write_word _ _ _ _ _ _ = _ |- _ ] => 
+            eapply (MEVAL.WriteCorrect meval_correct) with (cs := cs) (stn_m := (s0,s1)) in H; eauto
+        end.
+        destruct (WriteWord s0 (Mem s1) (evalLoc s1 l) valD); try contradiction.
+        eexists; split; [ reflexivity | ]. intuition.
+
+        generalize SEP.sheapD_pures. unfold SEP.ST.satisfies. intro XXX. 
+        rewrite sepFormula_eq in H3. unfold sepFormula_def in H3. simpl in *.
+        specialize (@XXX _ _ _ _ preds _ _ cs meta_env vars_env s3 H3). 
+        apply AllProvable_app' in H5. apply AllProvable_app; intuition auto.
+    Qed.
+
+    Lemma sym_evalInstr_correct' : forall instr stn_st instrD cs ss ss',
+      stateD funcs preds meta_env vars_env cs stn_st ss ->
+      sym_instrD funcs meta_env vars_env instr = Some instrD ->
+      sym_evalInstr Prover meval facts instr ss = Some ss' ->
+      exists st',
+        evalInstr (fst stn_st) (snd stn_st) instrD = Some st' /\
+        stateD funcs preds meta_env vars_env cs (fst stn_st, st') ss'.
+    Proof.
+      Opaque stateD.
+      destruct instr; unfold funcs in *; t_correct; simpl.
+      eapply sym_evalRval_correct in H1; eauto; simpl in *.
+      destruct H1. intuition.
+      eapply sym_evalLval_correct in H2; eauto; simpl in *.
+      destruct H2. intuition. unfold funcs in *; t_correct; eauto.
+
+      repeat match goal with
+               | [ H : _ |- _ ] => progress fold funcs in H
+               | [ H : exists x, _ |- _ ] => destruct H
+               | [ H : _ /\ _ |- _ ] => destruct H 
+               | [ H : sym_rvalueD _ _ _ _ = _ |- _ ] =>
+                 eapply sym_evalRval_correct in H; eauto
+             end.
+      
+      destruct b; eapply sym_evalLval_correct in H3; eauto; unfold funcs in *; t_correct; eauto.
+    Qed.
+
+    Lemma sym_assertTest_correct' : forall cs r rD t l lD ss stn_st,
+      stateD funcs preds meta_env vars_env cs stn_st ss ->
+      sym_rvalueD funcs meta_env vars_env r = Some rD ->
+      sym_rvalueD funcs meta_env vars_env l = Some lD ->
+      match Structured.evalCond rD t lD (fst stn_st) (snd stn_st) with
+        | None =>
+          forall res, 
+            match sym_assertTest Prover meval facts r t l ss res with
+              | Some _ => False
+              | None => True
+            end
+        | Some res' =>
+          match sym_assertTest Prover meval facts r t l ss res' with
+            | Some b => 
+              Provable funcs meta_env vars_env b
+            | None => True
+          end
+      end.
+    Proof.
+      unfold sym_assertTest; unfold Structured.evalCond; intros;
+        repeat match goal with
+                 | [ |- context [ sym_evalRval ?A ?B ?F ?X ?Y ] ] =>
+                   case_eq (sym_evalRval A B F X Y); intros
+                 | [ |- match ?X with 
+                          | None => True
+                          | Some _ => True
+                        end ] => destruct X; trivial
+               end.
+      case_eq (sym_evalRval Prover meval facts l ss); 
+        case_eq (sym_evalRval Prover meval facts r ss); intros;
+          try solve [ match goal with
+                        | [ |- match ?X with
+                                 | Some _ => _ | None => _ 
+                               end ] => destruct X; intros
+                      end;
+          repeat match goal with
+                   | [ H : _ = _ |- _ ] => rewrite H
+                   | [ |- context [ match ?X with 
+                                      | true => _ | false => _ 
+                                    end ] ] => destruct X
+                   | [ |- context [ match ?X with 
+                                      | IL.Eq => _ | Ne => _ | IL.Lt => _ | Le => _ 
+                                    end ] ] => destruct X
+                 end; trivial ].
+      repeat match goal with
+               | [ H : sym_rvalueD _ _ _ _ = Some _ |- _ ] =>
+                 generalize H ; eapply sym_evalRval_correct in H; eauto
+               | [ H : exists x, _ |- _ ] => destruct H
+               | [ H : _ /\ _ |- _ ] => destruct H
+               | [ H : _ = _ |- _ ] => rewrite H
+             end. intros.
+      unfold Provable; destruct t;
+        repeat (trivial; simpl;
+          match goal with
+            | [ |- context [ match ?X with
+                               | true => _
+                               | false => _
+                             end ] ] => 
+            case_eq X; intros
+            | [ H : exists x, _ |- _ ] => destruct H
+            | [ H : _ /\ _ |- _ ] => destruct H
+            | [ H : _ = _ |- _ ] => rewrite H
+          end);
+        unfold funcs in *; simpl in *;
+          repeat match goal with 
+                   | [ H : exprD _ _ _ _ _ = _ |- _ ] => rewrite H
+                   | [ H : @eq bool (?F _ _) _ |- _ ] => revert H ; clear ; unfold F ; intros
+                 end; simpl;
+          repeat match goal with
+                   | [ H : match ?X with 
+                             | left _ => _
+                             | right _ => _ 
+                           end = _ |- _ ] => destruct X; try congruence
+                 end;
+      eauto 10 using eq_le, lt_le, le_neq_lt.
+    Qed.
+  End typed.
+
+
+  Section typed2.
+    Variable ts : list type.
+    Let types := repr bedrock_types_r ts.
+
+    Local Notation "'pcT'" := (tvType 0).
+    Local Notation "'tvWord'" := (tvType 0).
+    Local Notation "'stT'" := (tvType 1).
+    Local Notation "'tvState'" := (tvType 2).
+    Local Notation "'tvTest'" := (tvType 3).
+    Local Notation "'tvReg'" := (tvType 4).
+
+    Variable fs : functions types.
+    Let funcs := repr (bedrock_funcs_r ts) fs.
+    Variable preds : SEP.predicates types pcT stT.
+
+    Variable Prover : ProverT types.
+    Variable PC : ProverT_correct Prover funcs.
+
+    Variable meval : MEVAL.MemEvaluator types pcT stT.
+    Variable meval_correct : MEVAL.MemEvaluator_correct meval funcs preds tvWord tvWord
+      (@IL_mem_satisfies ts) (@IL_ReadWord ts) (@IL_WriteWord ts).
+
+    Local Ltac t_correct := 
+      simpl; intros;
+        unfold IL_stn_st, IL_mem_satisfies, IL_ReadWord, IL_WriteWord in *;
+          repeat (simpl in *; 
+            match goal with
+              | [ H : Some _ = Some _ |- _ ] => inversion H; clear H; subst
+              | [ H : prod _ _ |- _ ] => destruct H
+              | [ H : match ?X with 
+                        | Some _ => _
+                        | None => _ 
+                      end |- _ ] =>
+              revert H; case_eq X; intros; try contradiction
+              | [ H : match ?X with 
+                        | Some _ => _
+                        | None => _ 
+                      end = _ |- _ ] =>
+              revert H; case_eq X; intros; try congruence
+              | [ H : _ = _ |- _ ] => rewrite H
+              | [ H : reg |- _ ] => destruct H
+            end; intuition); subst.
+
+    Lemma sym_evalInstrs_correct : forall (facts : Facts Prover) (meta_env var_env : env types),
+      Valid PC meta_env var_env facts  ->
+      forall is stn_st isD cs ss,
+        stateD funcs preds meta_env var_env cs stn_st ss ->
+        sym_instrsD funcs meta_env var_env is = Some isD ->
+        match evalInstrs (fst stn_st) (snd stn_st) isD with
+          | Some st' => 
+            match sym_evalInstrs Prover meval facts is ss with
+              | inl ss' => stateD funcs preds meta_env var_env cs (fst stn_st, st') ss'
+              | inr (ss', is') => 
+                match sym_instrsD funcs meta_env var_env is' with
+                  | None => False
+                  | Some is'D => 
+                    exists st'', stateD funcs preds meta_env var_env cs (fst stn_st, st'') ss' /\
+                      evalInstrs (fst stn_st) st'' is'D = Some st'
+                end
+            end
+          | None => 
+            match sym_evalInstrs Prover meval facts is ss with
+              | inl ss' => False
+              | inr (ss', is') => 
+                match sym_instrsD funcs meta_env var_env is' with
+                  | None => False
+                  | Some is'D => 
+                    exists st'', stateD funcs preds meta_env var_env cs (fst stn_st, st'') ss' /\
+                      evalInstrs (fst stn_st) st'' is'D = None
+                end
+            end
+        end.
+    Proof.
+      Opaque stateD.
+      induction is; simpl; intros;
+        repeat match goal with
+                 | [ H : Some _ = Some _ |- _ ] => inversion H; clear H; subst
+               end; simpl; destruct stn_st; simpl in *; eauto.
+
+      t_correct. simpl in *.
+      case_eq (evalInstr s s0 i); intros.
+      case_eq (sym_evalInstr Prover meval facts a ss); intros.      
+
+      Check sym_evalInstr_correct'.
+
+      destruct (@sym_evalInstr_correct' ts fs preds Prover PC meval meval_correct facts meta_env var_env
+        H a (s,s0) i cs ss s2 H0 H1 H4). simpl in *. intuition.
+      rewrite H6 in H3. inversion H3; clear H3; subst.
+      specialize (IHis (s, s1)). simpl in *. eapply IHis; eauto.
+      
+      simpl. rewrite H1. rewrite H2. simpl. 
+      case_eq (evalInstrs s s1 l); intros; exists s0; simpl; rewrite H3; eauto.
+
+      case_eq (sym_evalInstr Prover meval facts a ss); intros. 
+      Focus 2. simpl. rewrite H1. rewrite H2. exists s0; simpl; rewrite H3; intuition.
+
+      
+
+      edestruct (@sym_evalInstr_correct' ts fs preds Prover PC meval meval_correct facts meta_env var_env
+        H a (s,s0) i cs ss); eauto.
+      simpl in *. destruct H5. rewrite H3 in H5. congruence.
+      Transparent stateD.
+    Qed.
+
+    Variable learnHook : MEVAL.LearnHook types (SymState types pcT stT).
+    Variable learn_correct : @MEVAL.LearnHook_correct _ _ pcT stT learnHook (@stateD _ funcs preds) funcs preds.
+
+    Theorem evalStream_correct : forall sound_or_safe path stn uvars vars st,
+      istreamD funcs uvars vars path stn st sound_or_safe ->
+      forall cs ss,
+        stateD funcs preds uvars vars cs (stn,st) ss ->
+        forall facts, 
+          Valid PC uvars vars facts ->
+          let res := sym_evalStream Prover meval learnHook facts path ss in
+            match res with
+              | inl None => 
+                match sound_or_safe with
+                  | None => True
+                  | Some _ => False
+                end
+              | inl (Some ss') => 
+                match sound_or_safe with
+                  | None => False
+                  | Some st' => 
+                    Expr.forallEach (env_ext (length vars) (SymVars ss')) (fun venv =>
+                      let var_env := vars ++ venv in
+                        Expr.existsEach (env_ext (length uvars) (SymUVars ss')) (fun uenv' =>
+                          let meta_env := uvars ++ uenv' in 
+                            stateD funcs preds meta_env var_env cs (stn, st') ss'))
+                end
+              | inr (ss'', is') => 
+                exists st'' : state, 
+                  Expr.forallEach (env_ext (length vars) (SymVars ss'')) (fun venv =>
+                    let var_env := vars ++ venv in
+                      Expr.existsEach (env_ext (length uvars) (SymUVars ss'')) (fun uenv' =>
+                        let meta_env := uvars ++ uenv' in 
+                          istreamD funcs meta_env var_env is' stn st'' None
+                          /\ stateD funcs preds meta_env var_env cs (stn, st'') ss''))
+            end.
+    Proof.
+      revert learn_correct; revert PC; revert meval_correct. admit.
+(*
+    Opaque stateD.
+    induction path; simpl; intros;
+      repeat match goal with
+               | [ H : Some _ = Some _ |- _ ] => inversion H; clear H; subst
+             end; subst; eauto.
+    t_correct. destruct a; t_correct.
+        Focus.
+          eapply sym_evalInstrs_correct in H; eauto. simpl in *.
+          rewrite H4 in *.
+          revert H; case_eq (sym_evalInstrs Prover meval facts l ss); intros.
+          specialize (IHpath _ _ H5 _ _ H2 _ H1); eauto.
+          destruct p. simpl. destruct (sym_instrsD l1); try congruence.
+          destruct H2. destruct sound_or_safe; intuition eauto. contradiction.
+
+        Focus.
+          eapply sym_evalInstrs_correct in H; eauto; simpl in *.
+          rewrite H3 in *.
+          destruct (sym_evalInstrs facts l ss); try contradiction.
+          destruct p. simpl. destruct (sym_instrsD l1); try contradiction.
+          destruct H; intuition; destruct sound_or_safe; eauto.
+
+        Focus.
+          destruct s. revert H.
+          case_eq (sym_rvalueD s); case_eq (sym_rvalueD s0); intros; try contradiction.
+          destruct o.
+          generalize (sym_assertTest_correct facts _ _ t _ _ _ H0 H2 H b).
+          simpl. destruct H3. rewrite H3.
+          case_eq (sym_assertTest facts s t s0 ss b); intros.
+          eapply IHpath; eauto.
+          
+          destruct 
+*)
+    Admitted.
+  End typed2.
+
+
+(*
+  Section iface.
+    Variable ts : list type.
+    Let types := repr bedrock_types_r ts.
+
+    Local Notation "'pcT'" := (tvType 0).
+    Local Notation "'tvWord'" := (tvType 0).
+    Local Notation "'stT'" := (tvType 1).
+    Local Notation "'tvState'" := (tvType 2).
+    Local Notation "'tvTest'" := (tvType 3).
+    Local Notation "'tvReg'" := (tvType 4).
+
+    Theorem sym_evalInstr_correct : 
+      forall (fs : functions types) (preds : SEP.predicates types (tvType 0) (tvType 1)),
+        let funcs := repr (bedrock_funcs_r ts) fs in
+        forall (Prover : ProverT types) (PC : ProverT_correct Prover funcs)
+          (meval : MEVAL.MemEvaluator types (tvType 0) (tvType 1))
+          (meval_correct : MEVAL.MemEvaluator_correct meval funcs preds (tvType 0) (tvType 0)
+            (@IL_mem_satisfies ts) (@IL_ReadWord ts) (@IL_WriteWord ts)),
+      
+        forall (facts : Facts Prover) (meta_env var_env : env types) instr stn_st instrD cs ss ss',
+        Valid PC meta_env var_env facts  ->
+        stateD funcs preds meta_env var_env cs stn_st ss ->
+        sym_instrD funcs meta_env var_env instr = Some instrD ->
+        sym_evalInstr Prover meval facts instr ss = Some ss' ->
+        exists st',
+          evalInstr (fst stn_st) (snd stn_st) instrD = Some st' /\
+          stateD funcs preds meta_env var_env cs (fst stn_st, st') ss'.
+    Proof.
+      intros. eapply sym_evalInstr_correct'; eauto.
+    Qed.
+
+    Theorem sym_assertTest_correct : 
+      forall (fs : functions types) (preds : SEP.predicates types (tvType 0) (tvType 1)),
+        let funcs := repr (bedrock_funcs_r ts) fs in
+        forall (Prover : ProverT types) (PC : ProverT_correct Prover funcs)
+          (meval : MEVAL.MemEvaluator types (tvType 0) (tvType 1))
+          (meval_correct : MEVAL.MemEvaluator_correct meval funcs preds (tvType 0) (tvType 0)
+            (@IL_mem_satisfies ts) (@IL_ReadWord ts) (@IL_WriteWord ts)),
+          forall (facts : Facts Prover) (meta_env var_env : env types) cs r rD t l lD ss stn_st,
+            Valid PC meta_env var_env facts  ->
+            stateD funcs preds meta_env var_env cs stn_st ss ->
+            sym_rvalueD funcs meta_env var_env r = Some rD ->
+            sym_rvalueD funcs meta_env var_env l = Some lD ->
+              match Structured.evalCond rD t lD (fst stn_st) (snd stn_st) with
+                | None =>
+                  forall res, 
+                    match sym_assertTest Prover meval facts r t l ss res with
+                      | Some _ => False
+                      | None => True
+                    end
+                | Some res' =>
+                  match sym_assertTest Prover meval facts r t l ss res' with
+                    | Some b => 
+                      Provable funcs meta_env var_env b
+                    | None => True
+                  end
+              end.
+    Proof.
+      intros; eapply sym_assertTest_correct'; eauto.
+    Qed.
+  End iface.
+*)
+
+End SymIL_Correct.
+
