src/SymILTac.v
@@ -1,0 +1,1625 @@
+(** This file implements the tactics for symbolic evaluation for the
+ ** language defined in IL.v
+ **)
+Require Import IL SepIL SymIL SymILProofs.
+Require Import Word Memory.
+Require Import DepList EqdepClass.
+Require Import PropX.
+Require Import SepExpr SymEval.
+Require Import Expr.
+Require Import Prover.
+Require Import Env TypedPackage.
+Import List.
+
+Require Structured SymEval.
+Require Import ILEnv.
+
+Set Implicit Arguments.
+Set Strict Implicit.
+
+(*
+Add Rec LoadPath "/usr/local/lib/coq/user-contrib/" as Timing.  
+Add ML Path "/usr/local/lib/coq/user-contrib/". 
+Declare ML Module "Timing_plugin".
+*)
+
+(** The Symbolic Evaluation Interfaces *)
+Module MEVAL := SymIL.MEVAL.
+
+(** Unfortunately, most things can change while evaluating a stream,
+ ** so we have to move it outside the sections
+ **)
+Section stream_correctness.
+  Variable types' : list type.
+  Local Notation "'TYPES'" := (repr bedrock_types_r types').
+
+  Local Notation "'pcT'" := (tvType 0).
+  Local Notation "'tvWord'" := (tvType 0).
+  Local Notation "'stT'" := (tvType 1).
+  Local Notation "'tvState'" := (tvType 2).
+  Local Notation "'tvTest'" := (tvType 3).
+  Local Notation "'tvReg'" := (tvType 4).
+
+  Variable funcs' : functions TYPES.
+  Local Notation "'funcs'" := (repr (bedrock_funcs_r types') funcs').
+  Variable sfuncs : SEP.predicates TYPES pcT stT.
+
+  Variable meval : MEVAL.MemEvaluator TYPES pcT stT.
+  Variable meval_correct : MEVAL.MemEvaluator_correct meval funcs sfuncs tvWord tvWord 
+    (@SymIL.IL_mem_satisfies types') (@SymIL.IL_ReadWord types') (@SymIL.IL_WriteWord types').
+
+  Variable Prover : ProverT TYPES.
+  Variable PC : ProverT_correct Prover funcs.
+
+  Variable learnHook : MEVAL.LearnHook TYPES (SymIL.SymState TYPES pcT stT).
+  Variable learn_correct : @MEVAL.LearnHook_correct _ _ pcT stT learnHook (@stateD _ funcs sfuncs) funcs sfuncs.
+
+  Lemma ApplySymEval : forall uvars vars sound_or_safe path stn st,
+    istreamD funcs uvars vars path stn st sound_or_safe ->
+    forall cs ss,
+    stateD funcs sfuncs uvars vars cs (stn,st) ss ->
+    forall facts, 
+      Valid PC uvars vars facts ->
+      let res := sym_evalStream Prover meval learnHook facts path ss in
+      match res with
+        | inl None => 
+          match sound_or_safe with
+            | None => True
+            | Some _ => False
+          end
+        | inl (Some ss') => 
+          match sound_or_safe with
+            | None => False
+            | Some st' => 
+              Expr.forallEach (env_ext (length vars) (SymVars ss')) (fun venv =>
+                let var_env := vars ++ venv in
+                Expr.existsEach (env_ext (length uvars) (SymUVars ss')) (fun uenv' =>
+                  let meta_env := uvars ++ uenv' in 
+                  stateD funcs sfuncs meta_env var_env cs (stn, st') ss'))
+          end
+        | inr (ss'', is') => 
+          exists st'' : state, 
+            Expr.forallEach (env_ext (length vars) (SymVars ss'')) (fun venv =>
+              let var_env := vars ++ venv in
+              Expr.existsEach (env_ext (length uvars) (SymUVars ss'')) (fun uenv' =>
+                let meta_env := uvars ++ uenv' in 
+                     istreamD funcs meta_env var_env is' stn st'' None
+                  /\ stateD funcs sfuncs meta_env var_env cs (stn, st'') ss''))
+      end.
+  Proof.
+    (** This is really an exact duplicate of sym_evalStream_correct, it is here 
+     ** to set the order of arguments used by the tactic.
+     **)
+  Admitted.
+
+  Theorem stateD_proof_no_heap :
+    forall (uvars vars : Expr.env TYPES) (st : state) (sp rv rp : Expr.expr TYPES),
+      exprD funcs uvars vars sp tvWord = Some (Regs st Sp) ->
+      exprD funcs uvars vars rv tvWord = Some (Regs st Rv) ->
+      exprD funcs uvars vars rp tvWord = Some (Regs st Rp) ->
+      forall pures : list (Expr.expr TYPES),
+        Expr.AllProvable funcs uvars vars pures ->
+        forall (cs : codeSpec W (settings * state)) (stn : settings),
+          stateD funcs' sfuncs uvars vars cs (stn, st)
+          {| SymVars := map (@projT1 _ _) vars
+           ; SymUVars := map (@projT1 _ _) uvars
+           ; SymMem := None
+           ; SymRegs := (sp, rp, rv)
+           ; SymPures := pures
+          |}.
+  Proof.
+    unfold stateD. intros.
+    repeat match goal with
+             | [ H : _ = _ |- _ ] => rewrite H
+           end.
+    intuition auto.
+  Qed.
+
+  Theorem stateD_proof :
+    forall (uvars vars : Expr.env TYPES) (st : state) (sp rv rp : Expr.expr TYPES),
+      exprD funcs uvars vars sp tvWord = Some (Regs st Sp) ->
+      exprD funcs uvars vars rv tvWord = Some (Regs st Rv) ->
+      exprD funcs uvars vars rp tvWord = Some (Regs st Rp) ->
+      forall pures : list (Expr.expr TYPES),
+        Expr.AllProvable funcs uvars vars pures ->
+        forall (sh : SEP.sexpr TYPES pcT stT)
+          (hashed : SEP.SHeap TYPES pcT stT),
+          SEP.hash sh = (nil, hashed) ->
+          forall (cs : codeSpec W (settings * state)) (stn : settings),
+            interp cs (![SEP.sexprD funcs sfuncs uvars vars sh] (stn, st)) ->
+            stateD funcs' sfuncs uvars vars cs (stn, st)
+            {| SymVars := map (@projT1 _ _) vars
+             ; SymUVars := map (@projT1 _ _) uvars
+             ; SymMem := Some hashed
+             ; SymRegs := (sp, rp, rv)
+             ; SymPures := pures
+            |}.
+  Proof.
+    Opaque repr.
+    unfold stateD. intros.
+    repeat match goal with
+             | [ H : _ = _ |- _ ] => rewrite H
+           end.
+    generalize (SEP.hash_denote funcs sfuncs uvars cs sh vars). rewrite H3. simpl in *.
+    intro XX. rewrite <- XX. intuition eauto.
+    apply AllProvable_app; auto. rewrite XX in H4.
+    rewrite sepFormula_eq in H4. unfold sepFormula_def in H4.
+    eapply SEP.sheapD_pures.  
+    unfold SEP.ST.satisfies. simpl in *. eauto.
+  Qed.
+End stream_correctness.
+
+(** Reification **)
+
+(* Reify the instructions *)
+Ltac collectTypes_loc isConst l Ts :=
+  match l with
+    | Reg _ => Ts
+    | Imm ?i => collectTypes_expr isConst i Ts
+    | Indir _ ?i => collectTypes_expr isConst i Ts
+  end.
+Ltac reify_loc isConst l types funcs uvars vars k :=
+  match l with
+    | Reg ?r => 
+      let res := constr:(@SymReg types r) in
+        k uvars funcs res
+    | Imm ?i =>
+      reify_expr isConst i types funcs uvars vars ltac:(fun uvars funcs i =>
+        let l := constr:(@SymImm types i) in k uvars funcs l)
+    | Indir ?r ?i =>
+      reify_expr isConst i types funcs uvars vars ltac:(fun uvars funcs i =>
+        let l := constr:(@SymIndir types r i) in k uvars funcs l)
+  end.
+
+Ltac collectTypes_lvalue isConst l Ts :=
+  match l with
+    | LvReg _ => Ts
+    | LvMem ?l => collectTypes_loc isConst l Ts
+  end.
+Ltac reify_lvalue isConst l types funcs uvars vars k :=
+  match l with
+    | LvReg ?r => let l := constr:(@SymLvReg types r) in k uvars funcs l 
+    | LvMem ?l => 
+      reify_loc isConst l types funcs uvars vars ltac:(fun uvars funcs l =>
+        let l := constr:(@SymLvMem types l) in k uvars funcs l)
+  end.
+
+Ltac collectTypes_rvalue isConst r Ts :=
+  match r with
+    | RvLval ?l => collectTypes_lvalue isConst l Ts
+    | RvImm ?i => collectTypes_expr isConst i Ts
+    | RvLabel _ => let l := constr:(label:Type) in Reflect.cons_uniq l Ts
+  end.
+
+Ltac reify_rvalue isConst r types funcs uvars vars k :=
+  match r with
+    | RvLval ?l =>
+      reify_lvalue isConst l types funcs uvars vars ltac:(fun uvars funcs l =>
+        let l := constr:(@SymRvLval types l) in k uvars funcs l)
+    | RvImm ?i =>
+      reify_expr isConst i types funcs uvars vars ltac:(fun uvars funcs i =>
+        let l := constr:(@SymRvImm types i) in k uvars funcs l)
+    | RvLabel ?l => 
+      let r := constr:(@SymRvLabel types l) in k uvars funcs r
+  end.
+
+Ltac collectTypes_instr isConst i Ts :=
+  match i with
+    | Assign ?l ?r =>
+      let Ts := collectTypes_lvalue isConst l Ts in
+        collectTypes_rvalue isConst r Ts
+    | Binop ?l ?r1 _ ?r2 =>
+      let Ts := collectTypes_lvalue isConst l Ts in
+        let Ts := collectTypes_rvalue isConst r1 Ts in
+          collectTypes_rvalue isConst r2 Ts
+  end.
+Ltac reify_instr isConst i types funcs uvars vars k :=
+  match i with
+    | Assign ?l ?r =>
+      reify_lvalue isConst l types funcs uvars vars ltac:(fun uvars funcs l =>
+        reify_rvalue isConst r types funcs uvars vars ltac:(fun uvars funcs r =>
+          let res := constr:(@SymAssign types l r) in k uvars funcs res))
+    | Binop ?l ?r1 ?o ?r2 =>
+      reify_lvalue isConst l types funcs uvars vars ltac:(fun uvars funcs l =>
+        reify_rvalue isConst r1 types funcs uvars vars ltac:(fun uvars funcs r1 =>
+          reify_rvalue isConst r2 types funcs uvars vars ltac:(fun uvars funcs r2 =>
+            let res := constr:(@SymBinop types l r1 o r2) in k uvars funcs res)))
+  end.
+
+Ltac collectTypes_instrs isConst is Ts :=
+  match is with
+    | nil => Ts
+    | ?i :: ?is => 
+      let Ts := collectTypes_instr isConst i Ts in
+        collectTypes_instrs isConst is Ts
+  end.
+Ltac reify_instrs isConst is types funcs uvars vars k :=
+  match is with
+    | nil => 
+      let is := constr:(@nil (sym_instr types)) in k uvars funcs is
+    | ?i :: ?is =>
+      reify_instr isConst i types funcs uvars vars ltac:(fun uvars funcs i =>
+        reify_instrs isConst is types funcs uvars vars ltac:(fun uvars funcs is =>
+          let res := constr:(i :: is) in k uvars funcs res))
+  end.
+
+Ltac isConst e :=
+  match e with
+    | 0 => true
+    | S ?e => isConst e
+    | true => true
+    | false => true
+    | _ => false
+  end.
+
+Lemma Some_cong : forall A (x y : A),
+  x = y
+  -> Some x = Some y.
+  congruence.
+Qed.
+
+Ltac find_reg st r :=
+  match goal with
+    | [ H : Regs st r = ?x |- _ ] => constr:((x, Some_cong H))
+    | _ => constr:((Regs st r, @refl_equal (option W) (Some (Regs st r))))
+  end.
+
+Ltac open_stateD H0 :=
+  cbv beta iota zeta delta 
+    [ stateD Expr.exprD Expr.applyD
+      EquivDec.equiv_dec 
+      Expr.Range Expr.Domain Expr.Denotation
+      Expr.EqDec_tvar Expr.tvar_rec Expr.tvar_rect
+      sumbool_rec sumbool_rect
+      Peano_dec.eq_nat_dec nat_rec nat_rect eq_rec_r eq_rec eq_rect eq_sym
+      nth_error map value
+      f_equal
+
+      Expr.AllProvable Expr.Provable Expr.tvarD comparator
+    ] in H0; 
+    let a := fresh in 
+    let b := fresh in
+    let zz := fresh in destruct H0 as [ a [ b zz ] ] ;
+    destruct a as [ ? [ ? ? ] ];
+    repeat match type of zz with
+             | True => clear zz
+             | _ /\ _ => let v := fresh in destruct zz as [ v zz ]
+           end.
+
+Ltac get_instrs st :=
+  let rec find_exact H Hs :=
+    match Hs with
+      | tt => false
+      | H :: _ => true
+      | _ :: ?Hs => find_exact H Hs
+    end
+    in
+    let rec get_instrs st ignore :=
+      match goal with
+        | [ H : Structured.evalCond ?l _ ?r _ st = Some _ |- _ ] =>
+          match find_exact H ignore with
+            | false =>
+              let v := get_instrs st (H, ignore) in
+                constr:((((l,r), H), v))
+          end
+        | [ H : Structured.evalCond ?l _ ?r _ st = None |- _ ] =>
+          constr:((((l,r), H), tt))
+        | [ H : evalInstrs _ st ?is = Some ?X |- _ ] =>
+          let v := get_instrs X tt in
+            constr:(((is, H), v))
+        | [ H : evalInstrs _ st ?is = None |- _ ] =>
+          constr:(((is, H), tt))
+        | [ |- _ ] => tt
+      end
+      in get_instrs st tt.
+Ltac collectAllTypes_instrs is Ts :=
+  match is with
+    | tt => Ts
+    | (((?l,?r), _), ?is) =>
+      let Ts := collectTypes_rvalue ltac:(isConst) l Ts in
+        let Ts := collectTypes_rvalue ltac:(isConst) r Ts in
+          collectAllTypes_instrs is Ts
+    | ((?i, _), ?is) =>
+      let Ts := collectTypes_instrs ltac:(isConst) i Ts in
+        collectAllTypes_instrs is Ts
+  end.
+
+Ltac build_path types instrs st uvars vars funcs k :=
+  match instrs with
+    | tt => 
+      let is := constr:(nil : @istream types) in
+      let pf := constr:(refl_equal (Some st)) in
+      k uvars funcs is (Some st) pf
+    | ((?i, ?H), ?is) =>
+      match type of H with
+        | Structured.evalCond ?l ?t ?r _ ?st = ?st' =>
+          reify_rvalue ltac:(isConst) l types funcs uvars vars ltac:(fun uvars funcs l =>
+            reify_rvalue ltac:(isConst) r types funcs uvars vars ltac:(fun uvars funcs r =>
+              match st' with
+                | None => 
+                  let i := constr:(inr (@SymAssertCond types l t r st') :: (nil : @istream types)) in
+                  k uvars funcs i (@None state) H
+                | Some ?st'' => 
+                  build_path types is st uvars vars funcs ltac:(fun uvars funcs is sf pf =>
+                    let i := constr:(inr (@SymAssertCond types l t r st') :: is) in
+                    let pf := constr:(@conj _ _ H pf) in
+                    k uvars funcs i sf pf)
+              end))
+        | evalInstrs _ ?st _ = ?st' =>
+          reify_instrs ltac:(isConst) i types funcs uvars vars ltac:(fun uvars funcs sis =>
+            match st' with
+              | None => 
+                let i := constr:(inl (sis, None) :: (nil : @istream types)) in
+                  k uvars funcs i (@None state) H
+              | Some ?st'' =>
+                build_path types is st'' uvars vars funcs ltac:(fun uvars funcs is sf pf =>
+                  let i := constr:(inl (sis, st') :: is) in
+                  let pf := constr:(@conj _ _ H pf) in
+                  k uvars funcs i sf pf)
+            end)
+      end
+  end.
+
+Goal forall (cs : codeSpec W (settings * state)) (stn : settings) st st',
+  Structured.evalCond (RvImm (natToW 0)) IL.Eq (RvImm (natToW 0)) stn st' = Some true ->
+  evalInstrs stn st (Assign Rp (RvImm (natToW 0)) :: nil) = Some st' -> 
+  True.
+  intros.
+  match goal with
+    | [ |- _ ] => 
+      let i := get_instrs st in
+      let Ts := constr:(@nil Type) in
+      let Ts := collectAllTypes_instrs i Ts in
+      let types_ := eval unfold bedrock_types in bedrock_types in
+      let types_ := Expr.extend_all_types Ts types_ in
+      let typesV := fresh "types" in
+      pose (typesV := types_) ;
+      let v := constr:(nil : env typesV) in
+      let f := eval unfold ILEnv.bedrock_funcs in (ILEnv.bedrock_funcs typesV) in
+      build_path typesV i st v v f ltac:(fun uvars funcs is sf pf =>
+        assert (@istreamD typesV funcs uvars v is stn st sf)  by (exact pf))
+  end.
+  solve [ trivial ].
+Abort.
+
+Require Unfolder.
+Require Provers.
+Module UNF := Unfolder.Make SEP.
+Module PACKAGED := UNF.Packaged BedrockCoreEnv.
+Module PACK := PACKAGED.PACK.
+
+Module ILAlgoTypes <: AlgoTypes SEP BedrockCoreEnv.
+
+  Record AllAlgos (ts : list type) : Type :=
+  { Prover : option (ProverT (repr BedrockCoreEnv.core ts))
+  ; Hints : option (UNF.hintsPayload (repr BedrockCoreEnv.core ts) BedrockCoreEnv.pc BedrockCoreEnv.st)
+  ; MemEval : option (MEVAL.MemEvaluator (repr BedrockCoreEnv.core ts) BedrockCoreEnv.pc BedrockCoreEnv.st)
+  }.
+
+Section oplus.
+  Variable T : Type.
+  Variable F : T -> T -> T.
+
+  Definition oplus (l r : option T) : option T :=
+    match l , r with 
+      | None , _ => r
+      | _ , None => l
+      | Some l , Some r => Some (F l r)
+    end.
+End oplus.
+
+Definition AllAlgos_composite types (l r : AllAlgos types) : AllAlgos types :=
+  match l , r with
+    | {| Prover  := pl ; Hints := hl ; MemEval := ml |} , {| Prover := pr ; Hints := hr ; MemEval := mr |} =>
+      {| Prover  := oplus (@composite_ProverT _) pl pr 
+       ; Hints   := oplus (fun l r => {| UNF.Forward := UNF.Forward l ++ UNF.Forward r
+                                       ; UNF.Backward := UNF.Backward l ++ UNF.Backward r |}) hl hr
+       ; MemEval := oplus (@MEVAL.Composite.MemEvaluator_composite _ BedrockCoreEnv.pc BedrockCoreEnv.st) ml mr
+       |}
+  end.
+
+(*
+Fixpoint AllAlgos_composite_list types pc st (ls : list (AllAlgos types)) : AllAlgos types pc st :=
+  match ls with
+    | nil => {| Prover := None ; Hints := None ; MemEval := None |}
+    | l :: nil => l
+    | l :: ls =>
+      let r := AllAlgos_composite_list ls in
+      AllAlgos_composite l r
+  end.
+*)
+
+Record AllAlgos_correct
+  (types : list type)
+  (funcs : functions (repr BedrockCoreEnv.core types))
+  (preds : SEP.predicates (repr BedrockCoreEnv.core types) BedrockCoreEnv.pc BedrockCoreEnv.st)
+  (algos : AllAlgos types) : Type :=
+{ Acorrect_Prover :
+  match Prover algos with
+    | None => True
+    | Some P => ProverT_correct P funcs
+  end
+; Acorrect_Hints : 
+  match Hints algos with
+    | None => True
+    | Some H => UNF.hintsSoundness funcs preds H
+  end
+; Acorrect_MemEval :
+  match MemEval algos with
+    | None => True
+    | Some M => 
+      @MEVAL.MemEvaluator_correct _ BedrockCoreEnv.pc BedrockCoreEnv.st M funcs preds
+      (tvarD (repr BedrockCoreEnv.core types) BedrockCoreEnv.st) (tvType 0) (tvType 0) 
+      (@IL_mem_satisfies types) (@IL_ReadWord types) (@IL_WriteWord types)
+  end
+}.
+
+Theorem AllAlgos_correct_composite types (l r : AllAlgos types) funcs preds 
+  (CL : @AllAlgos_correct types funcs preds l)
+  (CR : @AllAlgos_correct types funcs preds r) :
+  @AllAlgos_correct types funcs preds (AllAlgos_composite l r).
+Proof.
+  destruct l; destruct r; destruct CL; destruct CR; simpl in *; constructor; simpl.
+  destruct Prover0; destruct Prover1; simpl; auto. apply composite_ProverT_correct; auto.
+  destruct Hints0; destruct Hints1; simpl; auto; destruct Acorrect_Hints0; destruct Acorrect_Hints1; constructor; simpl;
+    eapply Provers.Forall_app; auto.
+  destruct MemEval0; destruct MemEval1; simpl; auto. apply MEVAL.Composite.MemEvaluator_correct_composite; auto.
+Qed.
+
+(*
+Theorem AllAlgos_correct_composite_list types pc st (ls : list (AllAlgos types pc st)) funcs preds sat read write 
+  (C : @hlist (AllAlgos types pc st) (fun A => @AllAlgos_correct types pc st A funcs preds sat read write) ls) :
+  @AllAlgos_correct types pc st (AllAlgos_composite_list ls) funcs preds sat read write.
+Proof.
+  induction ls.
+  constructor; simpl; auto.
+
+  remember (a :: ls) as FOO. destruct C; inversion HeqFOO; subst.
+  simpl. destruct ls; auto.
+  apply AllAlgos_correct_composite; auto.
+Qed.
+*)
+
+Record TypedPackage : Type :=
+{ Env   : PACK.TypeEnv
+; Algos : forall ts, AllAlgos (PACK.applyTypes Env ts)
+; Algos_correct : forall ts fs ps,
+  @AllAlgos_correct (PACK.applyTypes Env ts) (PACK.applyFuncs Env _ fs) (PACK.applyPreds Env _ ps) (Algos ts)
+}.
+
+Definition EnvOf : TypedPackage -> PACK.TypeEnv := Env.
+
+Section unfolder_learnhook.
+  Variable types : list type.
+  Variable hints : UNF.hintsPayload (repr bedrock_types_r types) (tvType 0) (tvType 1).
+
+  Definition unfolder_LearnHook : MEVAL.LearnHook (repr bedrock_types_r types) 
+    (SymState (repr bedrock_types_r types) (tvType 0) (tvType 1)) :=
+    fun prover st facts => 
+      match SymMem st with
+        | Some m =>
+          match UNF.forward hints prover 10 facts
+            {| UNF.Vars := SymVars st 
+             ; UNF.UVars := SymUVars st
+             ; UNF.Heap := m
+            |}
+            with
+            | {| UNF.Vars := vs ; UNF.UVars := us ; UNF.Heap := m |} =>
+              {| SymVars := vs
+               ; SymUVars := us
+               ; SymMem := Some m
+               ; SymRegs := SymRegs st
+               ; SymPures := SymPures st ++ SEP.pures m
+               |}
+          end
+        | None => st
+      end.
+
+  Variable funcs : functions (repr bedrock_types_r types).
+  Variable preds : SEP.predicates (repr bedrock_types_r types) (tvType 0) (tvType 1).
+  Hypothesis hints_correct : UNF.hintsSoundness funcs preds hints.
+
+  Theorem unfolderLearnHook_correct 
+    : @MEVAL.LearnHook_correct (repr bedrock_types_r types) _ BedrockCoreEnv.pc BedrockCoreEnv.st (@unfolder_LearnHook) 
+    (@stateD _ funcs preds) funcs preds.
+  Proof.
+    unfold unfolder_LearnHook. econstructor.
+
+    destruct ss; simpl.
+    destruct SymMem; simpl; intros; subst; eauto.
+    generalize hints_correct.
+    admit.
+  Qed.
+  Transparent UNF.forward.
+End unfolder_learnhook.
+
+  Ltac unfolder_simplifier H := 
+    match H with
+      | tt => 
+        cbv delta [ 
+          UNF.Foralls UNF.Vars UNF.UVars UNF.Heap UNF.Hyps UNF.Lhs UNF.Rhs
+          UNF.Forward UNF.forward UNF.unfoldForward
+          UNF.Backward UNF.backward UNF.unfoldBackward
+          UNF.findWithRest UNF.find 
+          equiv_dec
+          UNF.substExpr UNF.substSexpr
+          Unfolder.FM.add
+
+          SEP.impures SEP.pures SEP.other
+          
+          Unfolder.allb andb
+
+          length map app
+          exprSubstU
+          
+          ExprUnify.exprUnifyArgs ExprUnify.empty_Subst 
+
+          unfolder_LearnHook
+          UNF.default_hintsPayload
+          UNF.fmFind
+          UNF.findWithRest'
+        ]
+      | _ => 
+        cbv delta [
+          UNF.Foralls UNF.Vars UNF.UVars UNF.Heap UNF.Hyps UNF.Lhs UNF.Rhs
+          UNF.Forward UNF.forward UNF.unfoldForward
+          UNF.Backward UNF.backward UNF.unfoldBackward
+          UNF.findWithRest UNF.find 
+          equiv_dec
+          UNF.substExpr UNF.substSexpr
+          Unfolder.FM.add
+
+          SEP.impures SEP.pures SEP.other
+          
+          Unfolder.allb andb
+
+          length map app
+          exprSubstU
+
+          ExprUnify.exprUnifyArgs ExprUnify.empty_Subst 
+
+          unfolder_LearnHook
+          UNF.default_hintsPayload
+          UNF.fmFind
+          UNF.findWithRest'
+        ] in H
+    end.
+
+(*
+Fixpoint drop A (ls : list A) (n : nat) : list A :=
+  match ls with
+    | nil => nil
+    | x :: ls' => match n with
+                    | O => ls
+                    | S n' => drop ls' n'
+                  end
+  end.
+*)
+
+Section apply_stream_correctness.
+  Variable types' : list type.
+  Local Notation "'TYPES'" := (repr bedrock_types_r types').
+
+  Local Notation "'pcT'" := BedrockCoreEnv.pc.
+  Local Notation "'tvWord'" := (tvType 0).
+  Local Notation "'stT'" := BedrockCoreEnv.st.
+  Local Notation "'tvState'" := (tvType 2).
+  Local Notation "'tvTest'" := (tvType 3).
+  Local Notation "'tvReg'" := (tvType 4).
+
+  Variable funcs' : functions TYPES.
+  Local Notation "'funcs'" := (repr (bedrock_funcs_r types') funcs').
+  Variable preds : SEP.predicates TYPES pcT stT.
+
+  Variable algos : AllAlgos TYPES.
+  Variable algos_correct : @AllAlgos_correct TYPES funcs preds algos.
+
+  (** Unfolding may have introduced some new variables, which we quantify existentially. *)
+  Fixpoint quantifyNewVars (vs : variables) (en : env TYPES) (k : env TYPES -> Prop) : Prop :=
+    match vs with
+      | nil => k en
+      | v :: vs' => exists x, quantifyNewVars vs' (en ++ existT _ v x :: nil) k
+    end.
+
+  Theorem Apply_sym_eval : forall stn uvars vars sound_or_safe st path,
+    let prover := match Prover algos with
+                    | None => Provers.reflexivityProver
+                    | Some p => p
+                  end in
+    let meval := match MemEval algos with
+                   | None => MEVAL.Default.MemEvaluator_default _ _ _ 
+                   | Some me => me
+                 end in
+    let unfolder := match Hints algos with
+                      | None => @MEVAL.LearnHookDefault.LearnHook_default _ _
+                      | Some h => unfolder_LearnHook h 
+                    end in
+    istreamD funcs uvars vars path stn st sound_or_safe ->
+    forall cs ss,
+      stateD funcs preds uvars vars cs (stn,st) ss ->
+      let facts := Summarize prover (match SymMem ss with
+                                       | None => SymPures ss
+                                       | Some m => SEP.pures m ++ SymPures ss
+                                     end) in
+      (** initial unfolding **)
+      let ss := unfolder prover ss facts in
+      let res := @sym_evalStream _ prover meval unfolder facts path ss in
+
+      match sound_or_safe with
+        | None =>
+          (** safe **)
+          match res with
+            | inl None => True
+            | inl (Some _) => False
+            | inr (ss'', is') => 
+              quantifyNewVars (skipn (length vars) ss''.(SymVars)) vars (fun vars =>                
+                exists st'' : state, 
+                  istreamD funcs uvars vars is' stn st'' None
+                  /\ stateD funcs preds uvars vars cs (stn, st'') ss'')
+            end
+        | Some st' =>
+          (** correct **)
+          match res with
+            | inl None => False                
+            | inl (Some ss') => quantifyNewVars (skipn (length vars) ss'.(SymVars)) vars (fun vars =>
+              stateD funcs preds uvars vars cs (stn, st') ss')
+            | inr (ss'', is') => 
+              quantifyNewVars (skipn (length vars) ss''.(SymVars)) vars (fun vars =>                
+                exists st'' : state, 
+                  istreamD funcs uvars vars is' stn st'' (Some st')
+                  /\ stateD funcs preds uvars vars cs (stn, st'') ss'')
+          end
+        end.
+  Proof.
+    generalize algos_correct. admit.
+(*
+    intros; eapply sym_eval_any; eauto.
+    Focus 3.
+
+    unfold facts. destruct PC. simpl. eapply Summarize_correct.
+    revert H0; clear.
+    destruct ss; destruct SymRegs0; destruct p; simpl; clear; intuition.
+    destruct SymMem0; auto.
+    eapply AllProvable_app; eauto.
+    
+    generalize SEP.sheapD_pures. unfold ST.satisfies.
+    intro XX.
+    rewrite sepFormula_eq in H0. unfold sepFormula_def in *.
+    simpl in *.S
+    specialize (XX _ (repr (bedrock_funcs_r types') funcs) (tvType 0) (tvType 1)); eauto. 
+*)
+  Qed.
+
+End apply_stream_correctness.
+
+Module SEP_REIFY := ReifySepExpr SEP.
+
+
+(** NOTE:
+ ** - [isConst] is an ltac function of type [* -> bool]
+ ** - [ext] is the extension. it is a value of type [TypedPackage]
+ ** - [simplifier] is an ltac that takes a hypothesis names and simplifies it
+ **     (this should be implmented using [cbv beta iota zeta delta [ ... ] in H])
+ **     (it is recommended/necessary to call [sym_evaluator] or import its simplification)
+ **)
+Check Algos_correct.
+Ltac sym_eval isConst ext simplifier :=
+(*  run_timer 100 ; *)
+  let rec init_from st :=
+    match goal with
+      | [ H : evalInstrs _ ?st' _ = Some st |- _ ] => init_from st'
+      | [ |- _ ] => st
+    end
+  in          
+  let shouldReflect P :=
+    match P with
+      | evalInstrs _ _ _ = _ => false
+      | Structured.evalCond _ _ _ _ _ = _ => false
+      | @PropX.interp _ _ _ _ => false
+      | @PropX.valid _ _ _ _ _ => false
+      | @eq ?X _ _ => 
+        match X with
+          | context [ PropX.PropX ] => false
+          | context [ PropX.spec ] => false
+        end
+      | forall x, _ => false
+      | exists x, _ => false
+      | _ => true
+    end
+  in
+  let stn_st_SF :=
+    match goal with
+      | [ H : interp _ (![ ?SF ] ?X) |- _ ] => 
+        let SF := eval unfold empB injB injBX starB exB hvarB in SF in
+        constr:((X, (SF, H)))
+      | [ H : Structured.evalCond _ _ _ ?stn ?st = _ |- _ ] => 
+        let st := init_from st in
+        constr:(((stn, st), tt))
+      | [ H : IL.evalInstrs ?stn ?st _ = _ |- _ ] =>
+        let st := init_from st in
+        constr:(((stn, st), tt))
+      | [ |- _ ] => tt
+    end
+  in
+  let cs :=
+    match goal with
+      | [ H : codeSpec _ _ |- _ ] => H
+    end
+  in
+  let reduce_repr sym ls :=
+    match sym with
+      | tt =>
+        eval cbv beta iota zeta delta [ 
+          ext
+          Env.repr_combine Env.listToRepr Env.listOptToRepr nil_Repr
+          PACK.Types PACK.Funcs PACK.Preds Env
+          PACK.applyTypes PACK.applyFuncs PACK.applyPreds
+          tl map repr
+          PACK.CE.core
+          bedrock_types_r bedrock_funcs_r
+        ] in ls
+      | _ => 
+        eval cbv beta iota zeta delta [
+          sym ext
+          Env.repr_combine Env.listToRepr Env.listOptToRepr nil_Repr
+          PACK.Types PACK.Funcs PACK.Preds Env
+          PACK.applyTypes PACK.applyFuncs PACK.applyPreds
+          map tl repr
+          PACK.CE.core
+          bedrock_types_r bedrock_funcs_r
+        ] in ls
+    end
+  in
+  let ext' := 
+    match ext with
+      | _ => eval cbv delta [ ext ] in ext
+      | _ => ext
+    end
+  in
+  match stn_st_SF with
+    | tt => idtac (* nothing to symbolically evluate *)
+    | ((?stn, ?st), ?SF) =>
+      match find_reg st Rp with
+        | (?rp_v, ?rp_pf) =>
+          match find_reg st Sp with
+            | (?sp_v, ?sp_pf) =>
+              match find_reg st Rv with
+                | (?rv_v, ?rv_pf) =>
+(*                  stop_timer 100 ; *)
+(*                  run_timer 101 ; *)
+                  let all_instrs := get_instrs st in
+                  let all_props := Expr.collect_props shouldReflect in
+                  let pures := Expr.props_types all_props in
+                  let regs := constr:((rp_v, (sp_v, (rv_v, tt)))) in
+(*                  stop_timer 101 ; *)
+                  (** collect the raw types **)
+(*                  run_timer 102 ; *)
+                  let Ts := constr:(@nil Type) in
+                  let Ts := 
+                    match SF with
+                      | tt => Ts
+                      | (?SF,_) => (** TODO: a little sketchy since it is in CPS **)
+                        SEP_REIFY.collectTypes_sexpr ltac:(isConst) SF Ts ltac:(fun Ts => Ts)
+                    end
+                  in
+                  let Ts := collectAllTypes_instrs all_instrs Ts in
+                    idtac Ts ; 
+                  let Ts := Expr.collectTypes_exprs ltac:(isConst) regs Ts in
+                    idtac Ts ; 
+                  let Ts := Expr.collectTypes_exprs ltac:(isConst) pures Ts in
+                    idtac Ts ;
+                  (** check for potential universe problems **)
+                  match Ts with
+                    | context [ PropX.PropX ] => 
+                      fail 1000 "found PropX in types list"
+                        "(this causes universe inconsistencies)" Ts
+                    | context [ PropX.spec ] => 
+                      fail 1000 "found PropX.spec in types list"
+                        "(this causes universe inconsistencies)" Ts
+                    | _ => idtac
+                  end;
+                  (** elaborate the types **)
+                  let types_ := reduce_repr tt (PACK.applyTypes (Env ext) nil) in
+                    idtac "<" types_ ; 
+                  let types_ := Expr.extend_all_types Ts types_ in
+                    idtac "-" ; 
+                  let typesV := fresh "types" in
+                  pose (typesV := types_);
+                  (** Check the types **)
+                  let pcT := constr:(tvType 0) in
+                  let stT := constr:(tvType 1) in
+                  (** build the variables **)
+                  idtac "XXX" ; 
+                  let uvars := constr:(@nil (@sigT Expr.tvar (fun t : Expr.tvar => Expr.tvarD typesV t))) in
+                  idtac "YYY" ; 
+                  let vars := uvars in
+                  (** build the base functions **)
+                  idtac "aaa" ; 
+                  let funcs := reduce_repr tt (PACK.applyFuncs (Env ext) typesV (repr (bedrock_funcs_r typesV) nil)) in
+                    idtac "<" funcs; 
+                   (** build the base sfunctions **)
+(*                  let preds := constr:(@nil (@SEP.ssignature typesV pcT stT)) in *)
+                    idtac ">" ;
+                  let preds := reduce_repr tt (PACK.applyPreds (Env ext) typesV nil) in
+                    idtac "<" preds ;
+                    idtac "pures = " pures ;
+                  (** reflect the expressions **)
+                  Expr.reify_exprs ltac:(isConst) pures typesV funcs uvars vars ltac:(fun uvars funcs pures =>
+                    idtac "C" ; 
+                  let proofs := Expr.props_proof all_props in
+                  Expr.reify_expr ltac:(isConst) rp_v typesV funcs uvars vars ltac:(fun uvars funcs rp_v =>
+                    idtac "D" ; 
+                  Expr.reify_expr ltac:(isConst) sp_v typesV funcs uvars vars ltac:(fun uvars funcs sp_v =>
+                    idtac "E" ;
+                  Expr.reify_expr ltac:(isConst) rv_v typesV funcs uvars vars ltac:(fun uvars funcs rv_v =>
+                    idtac "F" ; 
+                    let finish H syms :=
+                      let rec unfold_all syms :=
+                        match syms with
+                          | tt => idtac
+                          | (?X, ?Y) => unfold_all X ; unfold_all Y
+                          | ?X => subst X
+                        end
+                      in
+(*                      stop_timer 106 ; *)
+(*                      idtac "5" ;  *)
+(*                      run_timer 107 ; *)
+                      unfold_all syms ;
+(*                      stop_timer 107 ; *)
+(*                      idtac "6" ; *)
+(*                      run_timer 108 ; *)
+                      first [ simplifier H | fail 100000 "simplifier failed!" ]  ;
+(*                      stop_timer 108 ; *)
+(*                      run_timer 109 ;
+                      repeat match goal with
+                               | [ H : Logic.ex _ |- _ ] => destruct H
+                               | [ H : _ /\ _ |- _ ] => destruct H
+                               | [ H : True |- _ ] => clear H
+                               | [ H : ?E = ?E |- _ ] => clear H
+                               | _ => progress subst
+                             end;
+(*                      stop_timer 109 ; *)
+*)
+(*                      run_timer 110 ; *)
+                      ((try exact H) ||
+                       (let rec destruct_exs H :=
+                         match type of H with
+                           | Logic.ex _ => destruct H as [ ? H ] ; destruct_exs H
+                           | _ => destruct H as [ [ ? [ ? ? ] ] [ ? ? ] ]
+                         end
+                        in destruct_exs H)) 
+(*                      stop_timer 110 *)
+                    in
+                    build_path typesV all_instrs st uvars vars funcs ltac:(fun uvars funcs is fin_state is_pf =>
+                      idtac "0" ; 
+                      match SF with
+                        | tt => 
+(*                          stop_timer 102 ; *)
+                          let funcsV := fresh "funcs" in
+                          pose (funcsV := funcs) ;
+                          let predsV := fresh "preds" in
+                          pose (predsV := preds) ;
+(*                          let ExtC := constr:(@Algos_correct _ _ _ _ _ _ ext typesV funcsV predsV) in *)
+                          generalize (@stateD_proof_no_heap typesV funcsV predsV
+                            uvars vars st sp_v rv_v rp_v 
+                            sp_pf rv_pf rp_pf pures proofs cs stn) ;
+                          let H_stateD := fresh in
+                          intro H_stateD ;
+                          (apply (@Apply_sym_eval typesV funcsV predsV
+                            (@Algos ext typesV) (@Algos_correct ext typesV funcsV predsV)
+                            stn uvars vars fin_state st is is_pf) in H_stateD ;
+                           let syms := constr:((typesV, (funcsV, predsV))) in
+                           finish H_stateD syms) || fail 100000 "couldn't apply sym_eval_any! (non-SF case)"
+                        | (?SF, ?H_interp) =>
+                          idtac "1" funcs preds ; 
+                          SEP_REIFY.reify_sexpr ltac:(isConst) SF typesV funcs pcT stT preds uvars vars 
+                          ltac:(fun uvars funcs preds SF =>
+(*                            stop_timer 102 ; *)
+(*                            run_timer 103 ; *)
+                            idtac "2" ;  
+                            let funcsV := fresh "funcs" in
+                            pose (funcsV := funcs) ;
+                            let predsV := fresh "preds" in
+                            pose (predsV := preds) ;
+(*                            let ExtC := constr:(@Algos_correct ext typesV funcsV predsV) in *)
+(*                            stop_timer 103 ; *)
+(*                            run_timer 104 ; *)
+                            apply (@stateD_proof typesV funcsV predsV
+                              uvars vars _ sp_v rv_v rp_v 
+                              sp_pf rv_pf rp_pf pures proofs SF _ (refl_equal _)) in H_interp ;
+                            idtac "3" ; 
+(*                            stop_timer 104 ; *)
+(*                            run_timer 105 ; *)
+                            (apply (@Apply_sym_eval typesV funcsV predsV
+                              (@Algos ext typesV) (@Algos_correct ext typesV funcsV predsV)
+                              stn uvars vars fin_state st is is_pf) in H_interp ;
+(*                             stop_timer 105 ; *)
+(*                             run_timer 106 ; *)
+                             let syms := constr:((typesV, (funcsV, predsV))) in
+                             idtac "4" ; 
+                             finish H_interp syms) || 
+                            (idtac"couldn't apply sym_eval_any! (SF case)"; 
+                             first [ 
+                                 generalize (@Apply_sym_eval typesV funcsV predsV
+                                   (@Algos ext typesV) (@Algos_correct ext typesV funcsV predsV)
+                                   stn uvars vars fin_state st is is_pf) ; idtac "6" 
+                               | generalize (@Apply_sym_eval typesV funcsV predsV
+                                   (@Algos ext typesV) (@Algos_correct ext typesV funcsV predsV)
+                                   stn uvars vars fin_state st) ; idtac "5"  
+                               | generalize (@Apply_sym_eval typesV funcsV predsV
+                                   (@Algos ext typesV) (@Algos_correct ext typesV funcsV predsV)
+                                   stn uvars vars) ; idtac "4" 
+                               | generalize (@Apply_sym_eval typesV funcsV predsV
+                                   (@Algos ext typesV) (@Algos_correct ext typesV funcsV predsV)); idtac "3" 
+                               | generalize (@Apply_sym_eval typesV funcsV predsV
+                                   (@Algos ext typesV)) ; generalize (@Algos_correct ext typesV funcsV predsV) ; idtac "2" 
+                               | generalize (@Apply_sym_eval typesV funcsV predsV) ; idtac "1"  
+                             ])
+                            )
+                      end)))))
+              end
+          end
+      end
+  end.
+
+
+Ltac sym_evaluator H := 
+  unfolder_simplifier H ;
+  cbv beta iota zeta delta
+    [ sym_evalInstrs sym_evalInstr sym_evalLval sym_evalRval sym_evalLoc sym_evalStream sym_assertTest
+      sym_setReg sym_getReg
+      SEP.pures SEP.impures SEP.other
+      SymMem SymRegs SymPures SymVars SymUVars
+      SEP.star_SHeap SEP.liftSHeap SEP.multimap_join 
+      Expr.SemiDec_expr Expr.expr_seq_dec Expr.tvar_val_sdec Expr.Eq Expr.liftExpr
+
+      SEP.sheap_liftVars
+      app map nth_error value error fold_right hd hd_error tl tail rev
+      Decidables.seq_dec 
+      DepList.hlist_hd DepList.hlist_tl 
+      SepExpr.FM.find SepExpr.FM.add SepExpr.FM.remove SepExpr.FM.map SepExpr.FM.empty SepExpr.FM.fold
+      Compare_dec.lt_eq_lt_dec nat_rec nat_rect Peano_dec.eq_nat_dec sumbool_rec sumbool_rect
+      EquivDec.equiv_dec EquivDec.nat_eq_eqdec
+      f_equal 
+      bedrock_funcs_r bedrock_types
+      fst snd
+      Env.repr Env.updateAt 
+
+      stateD Expr.exprD 
+      Expr.applyD Expr.exprD Expr.Range Expr.Domain Expr.Denotation Expr.lookupAs
+      Expr.AllProvable Expr.AllProvable_gen Expr.Provable Expr.tvarD
+      SEP.sheapD SEP.starred SEP.sexprD
+      EquivDec.equiv_dec Expr.EqDec_tvar Expr.tvar_rec Expr.tvar_rect 
+      Logic.eq_sym eq_sym f_equal
+      eq_rec_r eq_rect eq_rec
+      nat_rec nat_rect
+      sumbool_rec sumbool_rect
+      
+      SEP.himp SEP.sexprD Expr.Impl 
+      Expr.applyD Expr.exprD Expr.Range Expr.Domain Expr.Denotation 
+      Expr.lookupAs
+      SEP.SDenotation SEP.SDomain
+      EquivDec.nat_eq_eqdec  
+      SEP.sheapD SEP.sepCancel
+      SEP.star_SHeap SEP.unify_remove_all 
+      SEP.multimap_join SEP.liftSHeap SEP.unify_remove SEP.starred 
+      Expr.tvarD Expr.Eq
+      
+      SepExpr.FM.fold SepExpr.FM.find SepExpr.FM.add SepExpr.FM.empty 
+      bedrock_types 
+        
+      Compare_dec.lt_eq_lt_dec Peano_dec.eq_nat_dec
+      SepExpr.FM.map ExprUnify.exprUnifyArgs ExprUnify.empty_Subst
+      ExprUnify.exprUnify ExprUnify.fold_left_2_opt 
+      EquivDec.equiv_dec Expr.EqDec_tvar Expr.tvar_rec Expr.tvar_rect 
+      ExprUnify.get_Eq
+      orb
+        
+      Expr.typeof comparator
+
+      fPlus fMinus fMult
+      
+      repr_combine default footprint repr' updateAt Default_signature nil_Repr EmptySet_type SEP.Default_predicate
+      bedrock_funcs_r bedrock_types_r
+
+      Summarize Learn Prove
+      
+      MEVAL.smemeval_read_word MEVAL.smemeval_write_word
+      
+      EquivDec_nat Peano_dec.eq_nat_dec
+
+      Prover.Prove Prover.Facts Prover.Learn Prover.Summarize
+
+      Hints Prover MemEval Env PACK.Funcs PACK.Types PACK.Preds Algos
+
+      (** expression unification **)
+      Compare_dec.lt_dec
+      Compare_dec.le_dec
+      Compare_dec.le_gt_dec
+      Compare_dec.le_lt_dec
+      Compare_dec.lt_eq_lt_dec
+
+      ExprUnify.Subst_lookup ExprUnify.Subst_replace ExprUnify.env_of_Subst
+      ExprUnify.get_Eq ExprUnify.exprUnifyArgs ExprUnify.exprUnify
+      ExprUnify.empty_Subst
+
+      ExprUnify.SUBST.empty
+      ExprUnify.SUBST.find
+      ExprUnify.SUBST.add
+      ExprUnify.SUBST.insert_at_right
+      ExprUnify.SUBST.remove
+      ExprUnify.SUBST.remove_add
+      ExprUnify.SUBST.find_add
+      ExprUnify.SUBST.fold
+      ExprUnify.SUBST.map
+
+      NatMap.Ordered_nat.compare
+      NatMap.Ordered_nat.eq_dec
+      Peano_dec.eq_nat_dec
+
+      ExprUnify.fold_left_2_opt ExprUnify.fold_left_3_opt
+      sumor_rec sumor_rect
+
+      (** unfolder should be unnecessary... **)
+      UNF.Vars UNF.UVars UNF.Heap 
+      UNF.Foralls UNF.Hyps UNF.Lhs UNF.Rhs 
+      UNF.Forward UNF.Backward 
+      UNF.forward UNF.unfoldForward UNF.findWithRest UNF.find
+      equiv_dec UNF.substExpr Unfolder.FM.add 
+      Unfolder.allb andb length map app exprSubstU ExprUnify.exprUnifyArgs
+      ExprUnify.empty_Subst unfolder_LearnHook
+      UNF.default_hintsPayload UNF.fmFind UNF.findWithRest'
+      UNF.findWithRest
+
+      SEP.hash SEP.star_SHeap SEP.liftSHeap SEP.multimap_join map UNF.substExpr UNF.substSexpr
+      rev_append
+
+      Unfolder.FM.fold Unfolder.FM.add
+
+      Unfolder.FM.empty
+      Unfolder.FM.find
+      Unfolder.FM.add
+      Unfolder.FM.insert_at_right
+      Unfolder.FM.remove
+      Unfolder.FM.remove_add
+      Unfolder.FM.find_add
+      Unfolder.FM.fold
+      Unfolder.FM.map
+
+      plus minus skipn quantifyNewVars Expr.Impl_ projT1 projT2
+    ] in H.
+
+Module EmptyPackage.
+  Definition empty_package : TypedPackage.
+  refine (
+    {| Env := {| PACK.Types := nil_Repr EmptySet_type
+               ; PACK.Funcs := fun ts => nil_Repr (Default_signature _)
+               ; PACK.Preds := fun ts => nil_Repr (SEP.Default_predicate _ _ _)
+               |} 
+     ; Algos := fun ts => {| Prover := None ; Hints := None ; MemEval := None |}
+     ; Algos_correct := _
+     |}).
+  abstract (constructor; simpl; trivial).
+  Defined.
+  
+
+  Ltac simplifier H :=
+    match H with
+      | tt => 
+        cbv delta [
+          empty_package UNF.default_hintsPayload
+        ]
+      | _ => 
+        cbv delta [
+          empty_package UNF.default_hintsPayload
+        ] in H
+    end ;
+    MEVAL.LearnHookDefault.unfolder H ;
+    Provers.unfold_reflexivityProver H ;
+    MEVAL.Default.unfolder H ;
+    sym_evaluator H.
+
+  Goal forall (cs : codeSpec W (settings * state)) (stn : settings) st st' SF,
+    PropX.interp cs (SepIL.SepFormula.sepFormula SF (stn, st)) -> 
+    Structured.evalCond (RvImm (natToW 0)) IL.Eq (RvImm (natToW 0)) stn st' = Some true ->
+    evalInstrs stn st (Assign Rp (RvImm (natToW 0)) :: nil) = Some st' -> 
+    Regs st' Rp = natToW 0.
+  Proof.
+   intros.
+   sym_eval ltac:(isConst) empty_package simplifier.
+   intuition congruence. 
+  Abort.
+
+End EmptyPackage.
+
+Module BedrockPackage.
+  Definition bedrock_package : TypedPackage.
+  refine (
+    {| Env := {| PACK.Types := nil_Repr EmptySet_type
+               ; PACK.Funcs := bedrock_funcs_r 
+               ; PACK.Preds := fun ts => nil_Repr (SEP.Default_predicate _ _ _)
+               |}
+     ; Algos := fun ts => {| Prover := None ; Hints := None ; MemEval := None |}
+     ; Algos_correct := _
+     |}).
+  abstract (constructor; simpl; trivial).
+  Defined.
+
+  Ltac simplifier H :=
+    match H with
+      | tt => 
+        cbv delta [
+          bedrock_package UNF.default_hintsPayload
+        ]
+      | _ => 
+        cbv delta [
+          bedrock_package UNF.default_hintsPayload
+        ] in H
+    end ;
+    MEVAL.LearnHookDefault.unfolder H ;
+    Provers.unfold_reflexivityProver H ;
+    MEVAL.Default.unfolder H ;
+    sym_evaluator H.
+End BedrockPackage.
+
+Module Package.
+
+Ltac build_prover_pack prover ret :=
+  let res := constr:( 
+    let env :=
+      {| PACK.Types := Prover.ProverTypes prover
+       ; PACK.Funcs := fun ts => 
+         nil_Repr (Default_signature (repr bedrock_types_r (repr (Prover.ProverTypes prover) ts)))
+       ; PACK.Preds := fun ts =>
+         nil_Repr (SEP.Default_predicate (repr bedrock_types_r (repr (Prover.ProverTypes prover) ts)) (tvType 0) (tvType 1))
+       |} 
+    in
+    let algos ts :=
+      @Build_AllAlgos (PACK.applyTypes env ts)
+         (Some (Prover.Prover prover (PACK.applyTypes env ts)))
+         None
+         None
+    in
+    {| Env := env
+     ; Algos := algos
+     ; Algos_correct := fun ts fs ps =>
+       let types := repr bedrock_types_r (repr (Prover.ProverTypes prover) ts) in
+       @Build_AllAlgos_correct types fs ps (algos ts)
+         (@Prover.Prover_correct prover types fs)
+         I I
+     |})
+  in
+  let res := eval simpl in res in
+  ret res.
+
+Goal TypedPackage.
+  build_prover_pack Provers.TransitivityProver ltac:(fun x => refine x).
+Defined.
+
+Check Build_AllAlgos_correct.
+
+Ltac build_mem_pack mem ret :=
+  match type of mem with
+    | @MEVAL.MemEvaluatorPackage ?tr ?pc ?st ?ptr ?val IL_mem_satisfies IL_ReadWord IL_WriteWord =>
+      (let res := constr:(
+        let TR := Env.repr_combine tr (MEVAL.MemEvalTypes mem) in
+        let env := 
+          {| PACK.Types := TR
+           ; PACK.Funcs := fun ts => MEVAL.MemEvalFuncs mem (Env.repr ILEnv.bedrock_types_r (Env.repr TR ts))
+           ; PACK.Preds := fun ts => MEVAL.MemEvalPreds mem (Env.repr ILEnv.bedrock_types_r (Env.repr TR ts))
+           |}
+        in
+        let algos ts :=
+          @Build_AllAlgos (PACK.applyTypes env ts) 
+             None
+             None 
+             (Some (MEVAL.MemEval mem (PACK.applyTypes env ts)))
+        in
+        @Build_TypedPackage env algos 
+          (fun ts fs ps => @Build_AllAlgos_correct _ _ _ (algos ts) I I
+            (MEVAL.MemEval_correct mem (Env.repr ILEnv.bedrock_types_r ts) _ _))) in
+      let res := eval simpl in res in
+      ret res) || fail 10000 "couldn't construct mem_package"
+    | ?T => 
+      fail 10000 "got bad type" T "expected value of type Packages.MemEvaluatorPackage"
+  end.
+
+Definition min_types_r : Repr type :=
+  {| footprint := firstn 2 (footprint bedrock_types_r)
+   ; default := default bedrock_types_r
+   |}.
+
+Goal TypedPackage.
+  pose (mem := 
+    {| MEVAL.MemEvalTypes := nil_Repr EmptySet_type
+     ; MEVAL.MemEvalFuncs := fun ts => nil_Repr (Default_signature _)
+     ; MEVAL.MemEvalPreds := fun ts => nil_Repr (SEP.Default_predicate _ _ _)
+     ; MEVAL.MemEval := fun ts => @MEVAL.Default.MemEvaluator_default _ (tvType 0) (tvType 1)
+     ; MEVAL.MemEval_correct := fun ts fs ps =>
+       @MEVAL.Default.MemEvaluator_default_correct _ _ _ _ _ _ _ _ _ _ _
+     |} : @MEVAL.MemEvaluatorPackage min_types_r (tvType 0) (tvType 1) (tvType 0) (tvType 0) IL_mem_satisfies IL_ReadWord IL_WriteWord).
+  build_mem_pack mem ltac:(fun x => refine x).
+Defined.
+
+(** builds a [TypedPackage] from the arguments
+ ** - [hints] is a list of separation logic hints
+ ** - [prover] is instance of [ProverT_correct]
+ ** - [mem] is a tuple of [forall ts fs ps, MemEvaluator_correct ts fs ps] plugin correct instances
+ **)
+Ltac build_hints_pack hints ret :=
+  let res := constr:(
+    let env :=
+      {| PACK.Types := PACKAGED.Types hints
+       ; PACK.Funcs := fun ts => PACKAGED.Functions hints (repr bedrock_types_r ts)
+       ; PACK.Preds := fun ts => PACKAGED.Predicates hints (repr bedrock_types_r ts) |}
+    in
+    let algos ts := 
+      @Build_AllAlgos (PACK.applyTypes env ts)
+        None 
+        (Some (PACKAGED.Hints hints ts))
+        None
+    in
+    @Build_TypedPackage env algos 
+     (fun ts fs ps => 
+       let types := repr bedrock_types_r (repr (PACKAGED.Types hints) ts) in
+       @Build_AllAlgos_correct _ _ _ (algos ts)
+         I (PACKAGED.HintsOk hints ts fs ps) I))
+  in
+  let res := eval simpl in res in
+  ret res.
+
+Definition bedrock_env : PACK.TypeEnv :=
+  {| PACK.Types := nil_Repr EmptySet_type
+   ; PACK.Funcs := fun ts => nil_Repr (Default_signature _)
+   ; PACK.Preds := fun ts => nil_Repr (SEP.Default_predicate _ _ _)
+  |}.
+
+Goal TypedPackage.
+  PACKAGED.prepareHints ltac:(fun x => x) W (prod IL.settings IL.state) ltac:(isConst) bedrock_env tt tt ltac:(fun v => 
+    build_hints_pack v ltac:(fun x => refine x)).
+Defined.
+
+
+(** given to [TypedPackage]s, combines them and passes the combined [TypedPackage]
+ ** to [k].
+ ** This tactic will fail if any of the environments are not compatible.
+ **)
+Ltac glue_pack l r ret :=
+  let res := constr:(
+    let ntypesV := Env.repr_combine (PACK.Types (Env l)) (PACK.Types (Env r)) in
+    let nfuncsV ts := 
+      Env.repr_combine (PACK.Funcs (Env l) (Env.repr ntypesV ts)) 
+                       (PACK.Funcs (Env r) (Env.repr ntypesV ts))
+    in
+    let npredsV ts :=
+      Env.repr_combine (PACK.Preds (Env l) (Env.repr ntypesV ts))
+                       (PACK.Preds (Env r) (Env.repr ntypesV ts))
+    in
+    let env :=
+      {| PACK.Types := ntypesV
+       ; PACK.Funcs := nfuncsV
+       ; PACK.Preds := npredsV
+       |}
+    in
+    let algos ts := 
+      AllAlgos_composite (Algos l (Env.repr ntypesV ts)) (Algos r (Env.repr ntypesV ts))
+    in
+    {| Env   := env 
+     ; Algos := algos 
+     ; Algos_correct := fun ts fs ps =>
+       AllAlgos_correct_composite (@Algos_correct l (Env.repr ntypesV ts)
+                                                    (Env.repr (nfuncsV ts) fs)
+                                                    (Env.repr (npredsV ts) ps))
+                                  (@Algos_correct r (Env.repr ntypesV ts)
+                                                    (Env.repr (nfuncsV ts) fs)
+                                                    (Env.repr (npredsV ts) ps))
+    |})
+  in ret res.
+
+(*
+Ltac refine_glue_pack l r :=
+  let reduce_repr e := e in
+  let opaque v k := k v in
+  match eval hnf in l with
+    | @Build_TypedPackage ?CT ?PC ?ST ?SAT ?READ ?WRITE ?tl ?fl ?pl ?al ?acl =>
+      match eval hnf in r with
+        | @Build_TypedPackage _ _ _ _ _ _ ?tr ?fr ?pr ?ar ?acr =>
+          refine (
+              let types := repr_combine tl tr in
+              let funcs := fun ts => repr_combine (fl (repr types ts)) (fr (repr types ts)) in
+              let preds := fun ts => repr_combine (pl (repr types ts)) (pr (repr types ts)) in
+              @Build_TypedPackage CT PC ST SAT READ WRITE 
+                types funcs preds
+                (fun ts => AllAlgos_composite (al (repr types ts)) (ar (repr types ts)))
+                _ 
+               ); 
+          (subst; abstract exact (fun ts fs ps => AllAlgos_correct_composite 
+                  (acl (repr (repr_combine tl tr) ts) 
+                       (repr (repr_combine (fl (repr (repr_combine tl tr) ts)) (fr (repr (repr_combine tl tr) ts))) fs)
+                       (repr (repr_combine (pl (repr (repr_combine tl tr) ts)) (pr (repr (repr_combine tl tr) ts))) ps))
+                  (acr (repr (repr_combine tl tr) ts)
+                       (repr (repr_combine (fl (repr (repr_combine tl tr) ts)) (fr (repr (repr_combine tl tr) ts))) fs)
+                       (repr (repr_combine (pl (repr (repr_combine tl tr) ts)) (pr (repr (repr_combine tl tr) ts))) ps))))
+      end
+  end.
+
+Ltac hlist_from_tuple tpl acc := 
+  match tpl with
+    | tt => acc
+    | (?L, ?R) => 
+      let acc := hlist_from_tuple R acc in
+      hlist_from_tuple L acc
+    | _ => constr:(@HCons _ _ _ _ tpl acc)
+  end.
+*)
+
+(** given a tuple or list of [TypedPackage]s, this tactic combines them all and calls [k] with 
+ ** the result.
+ **)
+Ltac glue_packs packs k :=
+  match type of packs with
+    | TypedPackage _ _ _ _ _ _ => k packs
+    | _ =>
+      match packs with
+        | tt => k BedrockPackage.bedrock_package
+        | nil => k BedrockPackage.bedrock_package
+        | ?L :: ?R =>
+          glue_packs R ltac:(fun R => glue_pack L)
+        | (?L, ?R) =>
+          glue_packs L ltac:(fun L => 
+          glue_packs R ltac:(fun R => 
+            glue_pack L R k))
+      end
+  end.
+
+(** TODO: is there a way to make this more efficient? **)
+Ltac opaque_pack pack :=
+  let pack := eval hnf in pack in
+  let pack := eval simpl in pack in
+  match pack with
+    | @Build_TypedPackage ?env ?algos ?pf =>
+      refine (@Build_TypedPackage env algos _); abstract (exact pf)
+  end.
+
+Goal TypedPackage.
+  build_prover_pack Provers.TransitivityProver ltac:(fun x => 
+    build_mem_pack (MEVAL.Default.package bedrock_types_r (tvType 0) (tvType 1) (tvType 0) (tvType 0) IL_mem_satisfies IL_ReadWord IL_WriteWord) ltac:(fun y =>   
+    glue_pack x y ltac:(opaque_pack))).
+Qed.
+
+(*
+Goal TypedPackage bedrock_types_r (tvType 0) (tvType 1) IL_mem_satisfies IL_ReadWord IL_WriteWord.
+  build_prover_pack Provers.TransitivityProver ltac:(fun x => 
+    build_mem_pack (MEVAL.Default.package bedrock_types_r (tvType 0) (tvType 1) (tvType 0) (tvType 0) IL_mem_satisfies IL_ReadWord IL_WriteWord) ltac:(fun y =>   
+      idtac "1" ;
+    glue_packs (x, y, y) ltac:(fun v => exact v))).
+Qed.
+*)
+End Package.
+Definition AlgoImpl := AllAlgos.
+Definition AlgoProof := AllAlgos_correct.
+End ILAlgoTypes.
+
+(**
+Module UnfolderLearnHook.
+  Require Unfolder.
+
+  Module UNF := Unfolder.Make BedrockHeap ST.
+
+  Section typed.
+    Variable types : list type.
+    Variable hints : UNF.hintsPayload (repr bedrock_types_r types) (tvType 0) (tvType 1).
+
+    Definition unfolder_LearnHook : MEVAL.LearnHook (repr bedrock_types_r types) 
+      (SymState (repr bedrock_types_r types) (tvType 0) (tvType 1)) :=
+      fun prover st facts => 
+        match SymMem st with
+          | Some m =>
+            match UNF.forward hints prover 10 facts
+              {| UNF.Vars := SymVars st 
+               ; UNF.UVars := SymUVars st
+               ; UNF.Heap := m
+              |}
+              with
+              | {| UNF.Vars := vs ; UNF.UVars := us ; UNF.Heap := m |} =>
+                {| SymVars := vs
+                 ; SymUVars := us
+                 ; SymMem := Some m
+                 ; SymRegs := SymRegs st
+                 ; SymPures := SymPures st
+                |}
+            end
+          | None => st
+        end.
+
+    Variable funcs : functions (repr bedrock_types_r types).
+    Variable preds : SEP.predicates (repr bedrock_types_r types) (tvType 0) (tvType 1).
+    Hypothesis hints_correct : UNF.hintsSoundness funcs preds hints.
+
+    Opaque UNF.forward.
+
+    Theorem unfolderLearnHook_correct 
+      : @MEVAL.LearnHook_correct (repr bedrock_types_r types) (tvType 0) (tvType 1) _ (@unfolder_LearnHook) 
+        (@stateD _ funcs preds) funcs preds.
+    Proof.
+      unfold unfolder_LearnHook. econstructor.
+
+      destruct ss; simpl.
+      destruct SymMem0; simpl; intros; subst; eauto.
+      generalize hints_correct.
+      admit.
+    Qed.
+    Transparent UNF.forward.
+  End typed.
+
+  Ltac unfolder_simplifier H := 
+    match H with
+      | tt => 
+        cbv delta [ 
+          UNF.Vars UNF.UVars UNF.Heap UNF.Lhs UNF.Rhs
+          UNF.Forward
+          UNF.forward
+          UNF.unfoldForward
+          UNF.findWithRest UNF.find 
+          equiv_dec
+          UNF.substExpr
+          Unfolder.FM.add
+
+          impures pures other
+          
+          Unfolder.allb 
+
+          length map app
+          exprSubstU
+          
+          ExprUnify.exprUnifyArgs ExprUnify.empty_Subst 
+
+          unfolder_LearnHook
+          UNF.default_hintsPayload
+          UNF.fmFind
+          UNF.findWithRest'
+        ]
+      | _ => 
+        cbv delta [ 
+          UNF.Vars UNF.UVars UNF.Heap UNF.Lhs UNF.Rhs
+          UNF.Forward
+          UNF.forward
+          UNF.unfoldForward
+          UNF.findWithRest UNF.find 
+          equiv_dec
+          UNF.substExpr
+          Unfolder.FM.add
+
+          impures pures other
+          
+          Unfolder.allb 
+
+          length map app
+          exprSubstU
+
+          ExprUnify.exprUnifyArgs ExprUnify.empty_Subst 
+
+          unfolder_LearnHook
+          UNF.default_hintsPayload
+          UNF.fmFind
+          UNF.findWithRest'
+        ] in H
+    end.
+
+  (** This ltac builds an unfolder given a hint database.
+   ** [hints] is a gallina term of type [forall ts fs pcT stT ps, UNF.hintsSoundness ts fs pcT stT ps H]
+   **   if [H] is the hints to use in unfolding
+   **)
+  Ltac unfolder_for hints :=
+    fun ts pc st fs ps => constr:(@unfolderLearnHook_correct ts _ fs ps (hints ts fs (tvType 0) (tvType 1) ps)).
+      
+  Goal forall (cs : codeSpec W (settings * state)) (stn : settings) st st' SF,
+    PropX.interp cs (SepIL.SepFormula.sepFormula SF (stn, st)) -> 
+    Structured.evalCond (RvImm (natToW 0)) IL.Eq (RvImm (natToW 0)) stn st' = Some true ->
+    evalInstrs stn st (Assign Rp (RvImm (natToW 0)) :: nil) = Some st' -> 
+    Regs st' Rp = natToW 0.
+  Proof.
+    intros.
+    Time sym_eval ltac:(isConst) 
+      ltac:(fun ts fs => constr:(@Provers.reflexivityProver_correct ts fs)) (* prover *)
+      ltac:(fun ts pc st fs ps k => let res := constr:(@Demo.demo_evaluator ts fs ps) in k tt res) (* memory evaluator *)
+      ltac:(unfolder_for (@UNF.hintsSoundness_default)) (* unfolder *)
+      ltac:(fun H => Provers.unfold_reflexivityProver H ; MEVAL.Default.unfolder H ; unfolder_simplifier H ; sym_evaluator H)
+      tt tt tt.
+    congruence.
+  Qed.
+
+End UnfolderLearnHook.
+**)
+
+(**
+Module PluginEvaluator.
+  
+  Definition plugin_evaluator ts (fs : functions (repr bedrock_types_r ts)) ps evals consistent_pf := 
+    @MEVAL.Plugin.PluginMemEvaluator_correct _ (tvType 0) (tvType 1) evals fs ps (settings * state) (tvType 0) (tvType 0)
+    (@IL_mem_satisfies ts)
+    (@IL_ReadWord ts)
+    (@IL_WriteWord ts)
+    consistent_pf.
+
+  (** This Ltac builds a function that can be instantiated to build a composite evaluator.
+   ** It should be applied to one argument and passed as the 3rd argument to [sym_eval].
+   ** Arguments:
+   ** - [known] is a tuple of [forall ts fs, @MemEvalPred_correct ts ? (tvType 0) (tvType 1) ? (tvType 0) (tvType 0) ... ]
+   **)
+  Ltac plugin_eval known :=
+    let rec find_in p ls acc :=
+      match ls with
+        | nil => fail 100000 " didn't find " p
+        | ?l :: ?ls =>
+          match Reflect.unifies (SDenotation l) p with
+            | true => acc
+            | false => 
+              find_in p ls (S acc)
+          end
+      end
+    in
+    fun ts _pc _st fs ps k =>
+      let psVal := eval hnf in ps in
+      let rec build_pf known k :=
+        match known with
+          | tt => 
+            let r := constr:(@nil (nat * MEVAL.Plugin.MemEvalPred (repr bedrock_types_r ts))) in
+            let pf := constr:(I) in
+            k r pf
+          | (?L, ?known) =>
+            let Z := type of L in
+            match type of L with
+              | forall ts,  forall fs, @MEVAL.Plugin.MemEvalPred_correct _ _ _ _ _ _ _ _ _ _ (@?s ts) _ =>
+                let p := eval simpl SDenotation in (SDenotation (s ts)) in
+                let idx := find_in p psVal 0 in                  
+                build_pf known ltac:(fun res pf =>
+                  let ZZZ := constr:(@L ts fs) in
+                  let E :=
+                    match type of ZZZ with
+                      | @MEVAL.Plugin.MemEvalPred_correct _ ?P _ _ _ _ _ _ _ _ _ _ => P
+                    end
+                  in
+                  let f := constr:((idx, E) :: res) in
+                  let pf := constr:(@conj _ _ ZZZ pf) in
+                  k f pf)              
+            end
+        end
+      in 
+      build_pf known ltac:(fun evals consistent_pf =>
+        let evalsV := fresh "evals" in
+        pose (evalsV := evals) ;
+        let consistentV := fresh "consistent" in
+          idtac "a" evals consistent_pf ;
+        let res := constr:(@plugin_evaluator ts fs ps evals consistent_pf) in
+          idtac "B" res;
+            pose res ;
+        k evalsV res).
+
+  Goal forall ts fs ps, 
+    { evals : _ & MEVAL.MemEvaluator_correct
+        (MEVAL.Plugin.MemEvaluator_plugin (tvType 0) (tvType 1) evals) fs ps
+        (tvType 0) (tvType 0) (@IL_mem_satisfies ts) (@IL_ReadWord ts) (@IL_WriteWord ts) }.
+  Proof.
+    intros.
+    plugin_eval tt ts (tvType 0) (tvType 1) fs ps ltac:(fun evals pf => econstructor; apply pf).
+
+
+forall (cs : codeSpec W (settings * state)) (stn : settings) st st' SF,
+    PropX.interp cs (SepIL.SepFormula.sepFormula SF (stn, st)) -> 
+    Structured.evalCond (RvImm (natToW 0)) IL.Eq (RvImm (natToW 0)) stn st' = Some true ->
+    evalInstrs stn st (Assign Rp (RvImm (natToW 0)) :: nil) = Some st' -> 
+    Regs st' Rp = natToW 0.
+  Proof.
+    intros.
+    Time sym_eval ltac:(isConst) 
+      ltac:(fun ts fs => constr:(@Provers.reflexivityProver_correct ts fs)) (* prover *)
+      ltac:(composite_eval tt) (* memory evaluator *)
+      ltac:(UnfolderLearnHook.unfolder_for (@UnfolderLearnHook.UNF.hintsSoundness_default)) (* unfolder *)
+      ltac:(fun H => Provers.unfold_reflexivityProver H ; MEVAL.Default.unfolder H ; UnfolderLearnHook.unfolder_simplifier H ; sym_evaluator H)
+      tt tt tt.
+    congruence.
+  Qed.
+
+End PluginEvaluator.
+**)
